Update nbg.lean

nbg/nbg.lean
@@ -1,3 +1,5 @@
+import tactic.interactive
+
 universes u v
 
 class nbg (α : Type u) (β : Type v) :=
@@ -42,7 +44,7 @@ class nbg (α : Type u) (β : Type v) :=
 (class_eq : β)
 (class_eq_prop : ∀ z, set_mem_class z class_eq ↔ ∃ x, z = set_pair (set_pair x x) (set_pair x x))
 
-theorem classical.dne (p : Prop) : ¬¬p → p
+theorem classical.dne {p : Prop} : ¬¬p → p
 | hp := or.cases_on (classical.em p) id (λ h, false.elim (hp h))
 
 theorem xor.not_right_of_left {p q : Prop} : xor p q → p → ¬q
@@ -57,6 +59,18 @@ theorem xor.not_left_of_right {p q : Prop} : xor p q → q → ¬p
 theorem xor.left_of_not_right {p q : Prop} : xor p q → ¬q → p
 | hpq hq := or.cases_on hpq (λ h, h.1) (λ h, false.rec p $ hq h.1)
 
+theorem forall_not_iff_not_exists {α : Sort u} {P : α → Prop} : (∀ a, ¬P a) ↔ (¬∃ a, P a) :=
+{ mp := λ hf he, Exists.cases_on he (λ a ha, hf a ha),
+  mpr := λ hne a ha, hne ⟨a, ha⟩ }
+
+theorem not_xor_iff_iff {p q : Prop} : ¬xor p q ↔ (p ↔ q) :=
+{ mp  := λ hnx,
+  { mp  := λ hp, (classical.dne $ λ hnq, hnx $ or.inl ⟨hp, hnq⟩),
+    mpr := λ hq, (classical.dne $ λ hnp, hnx $ or.inr ⟨hq, hnp⟩) },
+  mpr := λ hi hx, or.cases_on hx
+    (λ hpnq, hpnq.2 $ hi.1 hpnq.1)
+    (λ hqnp, hqnp.2 $ hi.2 hqnp.1) }
+
 namespace nbg
 
 variables {α : Type u} (β : Type v) [nbg α β] (x y z a b c d : α) (X Y Z A B C D : β)
@@ -64,6 +78,8 @@ variables {α : Type u} (β : Type v) [nbg α β] (x y z a b c d : α) (X Y Z A 
 def pair := set_pair β (set_pair β x x) (set_pair β x y)
 
 variables {β x y z a b c d X Y Z A B C D}
+
+notation x ∈ X := set_mem_class x X
 
 theorem set_pair_left : set_mem_set β x (set_pair β x y) :=
 begin
@@ -159,13 +175,13 @@ begin
   exact h_2
 end
 
-theorem class_int_ext : set_mem_class x X → set_mem_class x Y → set_mem_class x (class_int α X Y)
+theorem class_int_ext : x ∈ X → x ∈ Y → x ∈ (class_int α X Y)
 | hX hY := (class_int_prop X Y x).2 ⟨hX, hY⟩
 
-theorem class_prod_ext : set_mem_class x X → set_mem_class y Y → set_mem_class (pair β x y) (class_prod α X Y)
+theorem class_prod_ext : x ∈ X → y ∈ Y → set_mem_class (pair β x y) (class_prod α X Y)
 | hX hY := (class_prod_prop X Y (pair β x y)).2 ⟨x, y, hX, hY, rfl⟩
 
-theorem class_prod_left : set_mem_class (pair β x y) (class_prod α X Y) → set_mem_class x X
+theorem class_prod_left : set_mem_class (pair β x y) (class_prod α X Y) → x ∈ X
 | hxy :=
 begin
   have hab := (class_prod_prop X Y (pair β x y)).1 hxy,
@@ -175,7 +191,7 @@ begin
   exact left.symm ▸ h.1
 end
 
-theorem class_prod_right : set_mem_class (pair β x y) (class_prod α X Y) → set_mem_class y Y
+theorem class_prod_right : set_mem_class (pair β x y) (class_prod α X Y) → y ∈ Y
 | hxy :=
 begin
   have hab := (class_prod_prop X Y (pair β x y)).1 hxy,
@@ -185,8 +201,11 @@ begin
   exact right.symm ▸ h.2.1
 end
 
-theorem class_prod_split : set_mem_class (pair β x y) (class_prod α X Y) → set_mem_class x X ∧ set_mem_class y Y
+theorem class_prod_split : set_mem_class (pair β x y) (class_prod α X Y) → x ∈ X ∧ y ∈ Y
 | hxy := ⟨class_prod_left hxy, class_prod_right hxy⟩
+
+@[simp] theorem class_prod_iff : set_mem_class (pair β x y) (class_prod α X Y) ↔ x ∈ X ∧ y ∈ Y :=
+⟨class_prod_split, λ h, class_prod_ext h.1 h.2⟩
 
 theorem class_prod_comm_ext : set_mem_class (pair β x y) X → set_mem_class (pair β y x) (class_prod_comm α X)
 | hxy := (class_prod_comm_prop X (pair β y x)).2 ⟨x, y, hxy, rfl⟩
@@ -200,6 +219,9 @@ begin
   cases pair_ext h.2,
   exact left.symm ▸ right.symm ▸ h.1
 end
+
+@[simp] theorem class_prod_comm_iff : set_mem_class (pair β y x) (class_prod_comm α X) ↔ set_mem_class (pair β x y) X :=
+⟨class_prod_of_prod_comm, class_prod_comm_ext⟩
 
 theorem class_prod_comm'_ext : set_mem_class (pair β x (pair β y z)) X → set_mem_class (pair β y (pair β x z)) (class_prod_comm' α X)
 | hxyz := (class_prod_comm'_prop X (pair β y (pair β x z))).2 ⟨x, y, z, hxyz, rfl⟩
@@ -216,6 +238,9 @@ begin
   exact left.symm ▸ left_1.symm ▸ right_1.symm ▸ h.1
 end
 
+@[simp] theorem class_prod_comm'_iff : set_mem_class (pair β y (pair β x z)) (class_prod_comm' α X) ↔ set_mem_class (pair β x (pair β y z)) X :=
+⟨class_prod_of_prod_comm', class_prod_comm'_ext⟩
+
 theorem class_prod_assoc_ext : set_mem_class (pair β x (pair β y z)) X → set_mem_class (pair β (pair β x y) z) (class_prod_assoc α X)
 | hxyz := (class_prod_assoc_prop X (pair β (pair β x y) z)).2 ⟨x, y, z, hxyz, rfl⟩
 
@@ -230,6 +255,9 @@ begin
   cases pair_ext left,
   exact right.symm ▸ left_1.symm ▸ right_1.symm ▸ h.1
 end
+
+@[simp] theorem class_prod_assoc_iff : set_mem_class (pair β (pair β x y) z) (class_prod_assoc α X) ↔ set_mem_class (pair β x (pair β y z)) X :=
+⟨class_prod_of_prod_assoc, class_prod_assoc_ext⟩
 
 theorem class_prod_assoc'_ext : set_mem_class (pair β d (pair β a (pair β b c))) X → set_mem_class (pair β d (pair β (pair β a b) c)) (class_prod_assoc' α X)
 | habcd := (class_prod_assoc'_prop X _).2 ⟨a, b, c, d, habcd, rfl⟩
@@ -248,7 +276,10 @@ begin
   exact left.symm ▸ right_1.symm ▸ left_2.symm ▸ right_2.symm ▸ h.1
 end
 
-theorem class_range_ext : set_mem_class (pair β x y) X → set_mem_class y (class_range α X)
+@[simp] theorem class_prod_assoc'_iff : set_mem_class (pair β d (pair β (pair β a b) c)) (class_prod_assoc' α X) ↔ set_mem_class (pair β d (pair β a (pair β b c))) X :=
+⟨class_prod_of_prod_assoc', class_prod_assoc'_ext⟩
+
+theorem class_range_ext : set_mem_class (pair β x y) X → y ∈ (class_range α X)
 | hxy := (class_range_prop X y).2 ⟨x, hxy⟩
 
 theorem class_mem_ext : set_mem_set β x y → set_mem_class (pair β x y) (class_mem α β)
@@ -264,6 +295,9 @@ begin
   exact left.symm ▸ right.symm ▸ h.1
 end
 
+@[simp] theorem class_mem_iff : set_mem_class (pair β x y) (class_mem α β) ↔ set_mem_set β x y :=
+⟨class_mem_of_mem, class_mem_ext⟩
+
 theorem class_eq_ext : x = y → set_mem_class (pair β x y) (class_eq α β)
 | hxy := (class_eq_prop β (pair β x y)).2 ⟨x, hxy ▸ rfl⟩
 
@@ -276,25 +310,52 @@ begin
   exact right.symm ▸ left
 end
 
-theorem set_to_class_ext : set_mem_set β x y → set_mem_class x (set_to_class β y) :=
+@[simp] theorem class_eq_iff : set_mem_class (pair β x y) (class_eq α β) ↔ x = y :=
+⟨class_eq_of_eq, class_eq_ext⟩
+
+theorem set_to_class_ext : set_mem_set β x y → x ∈ (set_to_class β y) :=
 (set_to_class_prop β y x).1
 
-theorem class_mem_of_to_class : set_mem_class x (set_to_class β y) → set_mem_set β x y :=
+theorem class_mem_of_to_class : x ∈ (set_to_class β y) → set_mem_set β x y :=
 (set_to_class_prop β y x).2
 
+@[simp] theorem set_to_class_iff : x ∈ (set_to_class β y) ↔ set_mem_set β x y :=
+⟨class_mem_of_to_class, set_to_class_ext⟩
+
+theorem class_comp_prop1 : x ∈ (class_comp α X) ↔ ¬x ∈ X :=
+⟨(class_comp_prop X x).not_left_of_right, (class_comp_prop X x).right_of_not_left⟩
+
+theorem class_comp_prop2 : x ∈ X ↔ ¬x ∈ (class_comp α X) :=
+⟨(class_comp_prop X x).not_right_of_left, (class_comp_prop X x).left_of_not_right⟩
+
+variables (α X)
+
+def class_prod_assoc'' : β := (class_prod_comm α $ class_prod_assoc α $ class_prod_comm α $ class_prod_assoc α $ class_prod_comm α X)
+
+variables {α X}
+
+@[simp] theorem class_prod_assoc''_iff : set_mem_class (pair β x (pair β y z)) (class_prod_assoc'' α X) ↔ set_mem_class (pair β (pair β x y) z) X :=
+begin
+  unfold class_prod_assoc'',
+  rw class_prod_comm_iff,
+  rw class_prod_assoc_iff,
+  rw class_prod_comm_iff,
+  rw class_prod_assoc_iff,
+  rw class_prod_comm_iff
+end
+
 variables (α β)
+
 def class_univ : β := class_comp α (set_to_class β (set_empty α β))
+
 variables {α β}
 
-theorem class_univ_prop : set_mem_class x (class_univ α β) :=
+theorem class_univ_prop : x ∈ (class_univ α β) :=
 begin
-  cases class_comp_prop (set_to_class β (set_empty α β)) x,
-  cases h,
-  exfalso,
-  rw ←set_to_class_prop at h_left,
-  apply (set_empty_prop β) x, exact h_left,
-  cases h,
-  exact h_left
+  unfold class_univ,
+  rw class_comp_prop1,
+  rw set_to_class_iff,
+  apply set_empty_prop
 end
 
 theorem no_set_univ : ¬∃ x:α, ∀ y, set_mem_set β y x :=
@@ -337,6 +398,12 @@ end
 instance : has_emptyc α := ⟨set_empty α β⟩
 instance : has_union α := ⟨λ x y, set_union β $ set_pair β x y⟩
 
+@[simp] lemma univ_and (p : Prop) : x ∈ class_univ α β ∧ p ↔ p :=
+and_iff_right class_univ_prop
+
+@[simp] lemma and_univ (p : Prop) : p ∧ x ∈ class_univ α β ↔ p :=
+and_iff_left class_univ_prop
+
 variables (β x)
 
 def singleton : α := set_pair β x x
@@ -358,32 +425,23 @@ def contains_set : β := class_range α (class_int α (class_prod α (set_to_cla
 
 variables {β x}
 
-theorem contains_set_prop : set_mem_class x (contains_set β c) ↔ set_mem_set β c x :=
+theorem contains_set_prop : x ∈ (contains_set β c) ↔ set_mem_set β c x :=
 begin
   unfold contains_set,
   rw class_range_prop,
   split,
   intro h,
   cases h with z hz,
+  rw ←pair at hz,
   rw class_int_prop at hz,
-  cases hz,
-  rw class_prod_prop at hz_left,
-  cases hz_left with p hp,
-  cases hp with q h,
-  cases h with hp' h,
-  cases h with hp h,
-  cases pair_ext h,
-  rw [←left, ←right] at *,
-  rw ←set_to_class_prop at hp',
-  rw singleton_prop at hp',
-  rw ←hp',
-  rw class_mem_prop at hz_right,
-  cases hz_right with r hr,
-  cases hr with s hr,
-  cases hr with hr1 hr2,
-  cases pair_ext hr2,
-  rw [←left_1, ←right_1] at *,
-  exact hr1,
+  cases hz with h1 h2,
+  rw class_prod_iff at h1,
+  cases h1 with h3 h4,
+  rw set_to_class_iff at h3,
+  rw singleton_prop at h3,
+  rw h3 at *,
+  rw class_mem_iff at h2,
+  exact h2,
   intro hx,
   existsi c,
   apply class_int_ext,
@@ -399,13 +457,123 @@ variables (α β)
 
 def class_ne : β := class_int α (class_prod α (class_univ α β) (class_univ α β)) (class_comp α (class_eq α β))
 
+def class_not_mem : β := class_int α (class_prod α (class_univ α β) (class_univ α β)) (class_comp α (class_mem α β))
+
 variables {α β}
 
-theorem class_comp_prop1 : set_mem_class x (class_comp α X) ↔ ¬set_mem_class x X :=
-⟨(class_comp_prop X x).not_left_of_right, (class_comp_prop X x).right_of_not_left⟩
+theorem class_ne_ext : x ≠ y → set_mem_class (pair β x y) (class_ne α β)
+| hxy :=
+begin
+  unfold class_ne,
+  apply class_int_ext,
+  apply class_prod_ext class_univ_prop class_univ_prop,
+  rw class_comp_prop1,
+  rw class_eq_iff,
+  exact hxy
+end
 
-theorem class_comp_prop2 : set_mem_class x X ↔ ¬set_mem_class x (class_comp α X) :=
-⟨(class_comp_prop X x).not_right_of_left, (class_comp_prop X x).left_of_not_right⟩
+theorem class_ne_of_ne : set_mem_class (pair β x y) (class_ne α β) → x ≠ y
+| hxy :=
+begin
+  unfold class_ne at hxy,
+  rw class_int_prop at hxy,
+  cases hxy with h1 h2,
+  rw class_comp_prop1 at h2,
+  rw class_eq_iff at h2,
+  exact h2
+end
+
+@[simp] theorem class_ne_iff : set_mem_class (pair β x y) (class_ne α β) ↔ x ≠ y :=
+⟨class_ne_of_ne, class_ne_ext⟩
+
+
+theorem class_not_mem_ext : ¬set_mem_set β x y → set_mem_class (pair β x y) (class_not_mem α β)
+| hxy :=
+begin
+  unfold class_not_mem,
+  apply class_int_ext,
+  apply class_prod_ext class_univ_prop class_univ_prop,
+  rw class_comp_prop1,
+  rw class_mem_iff,
+  exact hxy
+end
+
+theorem class_not_mem_of_not_mem : set_mem_class (pair β x y) (class_not_mem α β) → ¬set_mem_set β x y
+| hxy :=
+begin
+  unfold class_not_mem at hxy,
+  rw class_int_prop at hxy,
+  cases hxy with h1 h2,
+  rw class_comp_prop1 at h2,
+  rw class_mem_iff at h2,
+  exact h2
+end
+
+@[simp] theorem class_not_mem_iff : set_mem_class (pair β x y) (class_not_mem α β) ↔ ¬set_mem_set β x y :=
+⟨class_not_mem_of_not_mem, class_not_mem_ext⟩
+
+variables (α X Y)
+
+def class_union : β := class_comp α (class_int α (class_comp α X) (class_comp α Y))
+
+def class_xor : β := class_union α (class_int α X (class_comp α Y)) (class_int α Y (class_comp α X))
+
+variables {α X Y}
+
+theorem class_union_ext : x ∈ X ∨ x ∈ Y → x ∈ (class_union α X Y)
+| hx :=
+begin
+  unfold class_union,
+  rw class_comp_prop1,
+  rw class_int_prop,
+  rw class_comp_prop1,
+  rw class_comp_prop1,
+  cases hx,
+  exact λ h, h.1 hx,
+  exact λ h, h.2 hx
+end
+
+theorem class_or_of_union : x ∈ (class_union α X Y) → x ∈ X ∨ x ∈ Y
+| hx :=
+begin
+  unfold class_union at hx,
+  rw class_comp_prop1 at hx,
+  rw class_int_prop at hx,
+  rw class_comp_prop1 at hx,
+  rw class_comp_prop1 at hx,
+  apply classical.dne,
+  exact λ h, hx ⟨λ hX, h $ or.inl hX, λ hY, h $ or.inr hY⟩
+end
+
+@[simp] theorem class_union_iff : x ∈ (class_union α X Y) ↔ x ∈ X ∨ x ∈ Y :=
+⟨class_or_of_union, class_union_ext⟩
+
+theorem class_xor_ext : xor (x ∈ X) (x ∈ Y) → x ∈ (class_xor α X Y)
+| hx :=
+begin
+  unfold class_xor,
+  rw class_union_iff,
+  rw class_int_prop,
+  rw class_int_prop,
+  rw class_comp_prop1,
+  rw class_comp_prop1,
+  exact hx
+end
+
+theorem class_xor_of_xor : x ∈ (class_xor α X Y) → xor (x ∈ X) (x ∈ Y)
+| hx :=
+begin
+  unfold class_xor at hx,
+  rw class_union_iff at hx,
+  rw class_int_prop at hx,
+  rw class_int_prop at hx,
+  rw class_comp_prop1 at hx,
+  rw class_comp_prop1 at hx,
+  exact hx
+end
+
+@[simp] theorem class_xor_iff : x ∈ (class_xor α X Y) ↔ xor (x ∈ X) (x ∈ Y) :=
+⟨class_xor_of_xor, class_xor_ext⟩
 
 variables (α β)
 
@@ -418,7 +586,7 @@ def class_singleton : β := class_int α (class_comp α (set_to_class β (single
 
 variables {α β}
 
-theorem class_singleton_prop : set_mem_class x (class_singleton α β) ↔ ∃ y, x = singleton β y :=
+theorem class_singleton_prop : x ∈ (class_singleton α β) ↔ ∃ y, x = singleton β y :=
 begin
   unfold class_singleton, unfold class_ne_mem,
   split,
@@ -541,19 +709,21 @@ def class_pair_singleton : β := class_int α (class_mem α β) (class_prod α (
 
 variables {α β}
 
-theorem class_pair_singleton_prop : set_mem_class z (class_pair_singleton α β) ↔ ∃ x y, y = singleton β x ∧ z = pair β x y :=
+theorem class_pair_singleton_prop : z ∈ (class_pair_singleton α β) ↔ ∃ x y, y = singleton β x ∧ z = pair β x y :=
 begin
   unfold class_pair_singleton,
-  rw class_int_prop,
-  rw class_mem_prop,
   split,
   intro h,
+  rw class_int_prop at h,
   cases h with h1 h3,
+  rw class_mem_prop at h1,
   cases h1 with x h1,
   cases h1 with y h1,
   cases h1 with h1 h2,
   rw h2 at *,
-  have h3 := (class_prod_split h3).2,
+  rw ←pair at h3,
+  rw class_prod_iff at h3,
+  rw and_iff_right class_univ_prop at h3,
   rw class_singleton_prop at h3,
   cases h3 with a ha,
   existsi a,
@@ -568,16 +738,13 @@ begin
   cases h with x h,
   cases h with y h,
   cases h with h1 h2,
-  split,
-  existsi x,
-  existsi y,
-  split,
-  rw h1,
-  rw singleton_prop,
-  exact h2,
+  apply class_int_ext,
   rw h2,
-  apply class_prod_ext,
-  apply class_univ_prop,
+  rw h1,
+  rw class_mem_iff,
+  rw singleton_prop,
+  rw h2,
+  apply class_prod_ext class_univ_prop,
   rw class_singleton_prop,
   existsi x,
   exact h1
@@ -636,5 +803,211 @@ begin
   rw h,
   rw class_singleton_prop
 end
+
+-- { (a,b) | b = a ∪ {a} }
+-- { (a,b) | ∀ c, c ∈ b ↔ c ∈ a ∨ c = a }
+-- { (a,b) | ¬ ∃ c, (c ∈ b ∧ c ∉ a ∧ c ≠ a) ∨ (c ∉ b ∧ (c ∈ a ∨ c = a)) }
+-- { (a,b) | ¬ ∃ c, c ∈ b ⊕ c ∈ a ∨ c = a }
+
+variables (β x)
+
+def succ : α := (set_union β $ set_pair β x $ singleton β x)
+
+variables {β x}
+
+variables (α β)
+
+def class_pair_succ : β := class_int α
+(class_prod α (class_univ α β) (class_univ α β))
+(class_comp α $ class_range α $ class_xor α
+  (class_prod_comm' α $ class_prod α (class_univ α β) (class_mem α β))
+  (class_prod_assoc'' α $ class_prod α (class_union α (class_mem α β) (class_eq α β)) (class_univ α β))
+)
+
+variables {α β}
+
+@[simp] theorem class_pair_succ_iff : set_mem_class (pair β x y) (class_pair_succ α β) ↔ y = succ β x :=
+begin
+  unfold class_pair_succ,
+  unfold succ,
+  split,
+  intro h,
+  rw class_int_prop at h,
+  rw class_prod_iff at h,
+  rw and_iff_right class_univ_prop at h,
+  rw and_iff_right class_univ_prop at h,
+  rw class_comp_prop1 at h,
+  rw class_range_prop at h,
+  rw ←forall_not_iff_not_exists at h,
+  apply set_ext y,
+  intro z,
+  split,
+  intro hzy,
+  rw set_union_prop,
+  specialize h z,
+  rw class_xor_iff at h,
+  rw not_xor_iff_iff at h,
+  rw ←pair at h,
+  cases h with h1 h2,
+  rw class_prod_comm'_iff at h1,
+  rw class_prod_iff at h1,
+  rw and_iff_right class_univ_prop at h1,
+  rw class_mem_iff at h1,
+  specialize h1 hzy,
+  rw class_prod_assoc''_iff at h1,
+  rw class_prod_iff at h1,
+  rw and_iff_left class_univ_prop at h1,
+  rw class_union_iff at h1,
+  cases h1 with hm he,
+  rw class_mem_iff at hm,
+  existsi x,
+  split,
+  exact hm,
+  exact set_pair_left,
+  rw class_eq_iff at he,
+  existsi singleton β x,
+  split,
+  rw singleton_prop,
+  exact he,
+  exact set_pair_right,
+  intro h1,
+  rw set_union_prop at h1,
+  cases h1 with t ht,
+  cases ht with hm hp,
+  specialize h z,
+  rw class_xor_iff at h,
+  rw not_xor_iff_iff at h,
+  rw ←pair at h,
+  cases h with h1 h2,
+  rw class_prod_comm'_iff at h2,
+  rw class_prod_iff at h2,
+  rw and_iff_right class_univ_prop at h2,
+  rw class_mem_iff at h2,
+  apply h2,
+  rw class_prod_assoc''_iff,
+  rw class_prod_iff,
+  rw and_iff_left class_univ_prop,
+  rw class_union_iff,
+  rw class_mem_iff,
+  rw class_eq_iff,
+  rw set_pair_prop at hp,
+  cases hp with he hm2,
+  rw ←he,
+  left,
+  exact hm,
+  rw hm2 at hm,
+  rw singleton_prop at hm,
+  right,
+  exact hm,
+  intro hy,
+  apply class_int_ext,
+  exact class_prod_ext class_univ_prop class_univ_prop,
+  rw class_comp_prop1,
+  intro hx,
+  rw class_range_prop at hx,
+  cases hx with z h1,
+  rw class_xor_iff at h1,
+  rw ←pair at h1,
+  rw class_prod_comm'_iff at h1,
+  rw class_prod_iff at h1,
+  rw class_prod_assoc''_iff at h1,
+  rw class_prod_iff at h1,
+  rw and_iff_right class_univ_prop at h1,
+  rw and_iff_left class_univ_prop at h1,
+  rw class_union_iff at h1,
+  rw class_mem_iff at h1,
+  rw class_mem_iff at h1,
+  rw class_eq_iff at h1,
+  rw hy at h1,
+  rw set_union_prop at h1,
+  cases h1 with h1 h1,
+  cases h1 with h1 h2,
+  cases h1 with t ht,
+  cases ht with h3 h4,
+  rw set_pair_prop at h4,
+  cases h4 with he hm,
+  rw he at h3,
+  apply h2,
+  left,
+  exact h3,
+  rw hm at h3,
+  rw singleton_prop at h3,
+  apply h2,
+  right,
+  exact h3,
+  cases h1 with h1 h2,
+  apply h2,
+  cases h1 with hm he,
+  existsi x,
+  split,
+  exact hm,
+  apply set_pair_left,
+  existsi singleton β x,
+  split,
+  rw singleton_prop,
+  exact he,
+  apply set_pair_right
+end
+
+variables (α β)
+
+-- { A | 0 ∈ A ∧ ∀ n, n ∈ A → succ (n) ∈ A }
+-- { A | 0 ∈ A ∧ ¬∃ n, n ∈ A ∧ succ (n) ∉ A }
+def class_inductive : β :=
+class_int α
+  (contains_set β (set_empty α β))
+  (class_comp α $ class_range α $ class_int α
+    (class_prod α (class_pair_succ α β) (class_univ α β))
+    (class_int α
+      (class_prod_assoc α $ class_prod_comm' α $ class_prod α (class_univ α β) (class_mem α β))
+      (class_prod_assoc α $ class_prod α (class_univ α β) (class_not_mem α β)) ) )
+
+variables {α β}
+
+@[simp] theorem class_inductive_iff : x ∈ (class_inductive α β) ↔ (set_mem_set β (set_empty α β) x ∧ ∀ y, set_mem_set β y x → set_mem_set β (succ β y) x) :=
+begin
+  unfold class_inductive,
+  rw class_int_prop,
+  rw class_comp_prop1,
+  rw class_range_prop,
+  rw contains_set_prop,
+  apply and_congr,
+  exact iff.rfl,
+  split,
+  intro h1,
+  intros z hz,
+  apply classical.dne,
+  intro hsz,
+  apply h1,
+  existsi pair β z (succ β z),
+  rw ←pair,
+  apply class_int_ext,
+  simp,
+  apply class_int_ext,
+  simpa,
+  simpa,
+  intros h h1,
+  cases h1 with y h1,
+  rw ←pair at h1,
+  rw class_int_prop at h1,
+  cases h1 with h1 h2,
+  rw class_int_prop at h2,
+  cases h2 with h2 h3,
+  have h4 := h1,
+  simp at h4,
+  unfold class_pair_succ at h4,
+  rw class_int_prop at h4,
+  rw class_prod_prop at h4,
+  cases h4.1 with u h5,
+  clear h4,
+  cases h5 with v h4,
+  rw ←pair at h4,
+  rw h4.2.2 at *,
+  clear h4,
+  simp at *,
+  exact (h1 ▸ h3) (h u h2),
+end
+
+-- ℕ = { n | ∀ A, ({} ∈ A ∧ ∀ n, n ∈ A → n ∪ {n} ∈ A) → n ∈ A }
 
 end nbg
